src/StAM.v
@@ -4,18 +4,14 @@ Record representing the AM Monad state structure.
 Author:  Adam Petz, ampetz@ku.edu
 *)
 
-Require Import Maps_Class.
+Require Import Maps.
 Require Import Coq.Arith.EqNat.
 
-(*Definition BS := nat. *)
-
-Instance nat_EqClass : EqClass nat :=
-  { eqb:= PeanoNat.Nat.eqb;
-    eqb_leibniz := beq_nat_true }.
+Definition BS := nat.
 
 (* Specific AM monad state *)
 Record AM_St : Type := mkAM_St
-                         { am_nonceMap : MapC nat nat;
+                         { am_nonceMap : MapC nat BS;
                            am_nonceId : nat;
                            checked : list nat }.
                                          
